revert changes in Exponentiation

code/experimental/rsa/Exponentiation.fst
@@ -6,53 +6,21 @@ open FStar.Int.Cast
 open FStar.All
 
 open Multiplication
+open Division
 open Convert
 
 module U32 = FStar.UInt32
 module U64 = FStar.UInt64
-module Div = Division
 
 type bignum = buffer FStar.UInt64.t
-type lbignum (len:U32.t) = 
-     b:bignum{length b = U32.v len} 
-
-type bnlen = (l:U32.t{U32.v l > 0 /\ U32.v l <= 8192})
-type exp_state (rLen:bnlen) (aLen:bnlen) = lbignum U32.(rLen +^ aLen +^ (2ul *^ aLen) +^ (aLen +^ rLen))
-
-let get_r_i #r #a (st:exp_state r a) : lbignum r = Buffer.sub st 0ul r
-let get_tmp #r #a (st:exp_state r a) : lbignum a = Buffer.sub st r a
-let get_tmp2 #r #a (st:exp_state r a) : lbignum U32.(2ul *^ a) = Buffer.sub st U32.(r +^ a) U32.(2ul *^ a)
-let get_r_itmp #r #a (st:exp_state r a) :lbignum U32.(a +^ r) = Buffer.sub st U32.(r +^ a +^ 2ul *^ a) U32.(a +^ r)
-
-let exp_state_inv r a (st:exp_state r a) = 
-           let r_i = get_r_i st in
-           let tmp = get_tmp st in
-           let tmp2 = get_tmp2 st in
-           let r_itmp = get_r_itmp st in
-           let r = frameOf r_i in
-	     r == frameOf tmp /\
-	     r == frameOf tmp2 /\
-	     r == frameOf r_itmp /\
-	     disjoint r_i tmp /\
-	     disjoint r_i tmp2 /\
-	     disjoint r_i r_itmp /\ 
-	     disjoint tmp tmp2 /\ 
-	     disjoint tmp r_itmp /\ 
-       	 disjoint tmp2 r_itmp 
-
-
-let exp_state_st_inv (rLen:bnlen) (aLen:bnlen) (st:exp_state rLen aLen) (h:FStar.HyperStack.mem) = 
-	     exp_state_inv rLen aLen st /\ live h st
-		       
 
 (* check if input[ind] is equal to 1 *)
 val bn_bit_is_set:
-    input:bignum ->
-    ind:U32.t{U32.v ind / 64 < length input} ->
+    input:bignum -> 
+    ind:U32.t{U32.v ind / 64 < length input} -> 
     Stack bool
     (requires (fun h -> live h input))
-    (ensures  (fun h0 _ h1 -> live h0 input /\ live h1 input /\ h0 == h1))
-
+    (ensures  (fun h0 r h1 -> live h0 input /\ live h1 input))
 let bn_bit_is_set input ind =
     let i = U32.(ind /^ 64ul) in
     let j = U32.(ind %^ 64ul) in
@@ -60,62 +28,63 @@ let bn_bit_is_set input ind =
     let res = U64.(((tmp >>^ j) &^ 1uL) =^ 1uL) in
     res
 
-
 val mod_exp_loop:
-    modBits:U32.t{U32.v modBits > 0} -> aLen:bnlen ->
-    bBits:U32.t{U32.v bBits > 0} -> resLen:bnlen ->
-    n:lbignum (bits_to_bn modBits) ->
-    b:lbignum (bits_to_bn bBits){disjoint n b} ->
-    count:U32.t{U32.v count <= length b} ->
-    st:exp_state resLen aLen{disjoint st n /\ disjoint st b} -> Stack unit
-    (requires (fun h -> live h n /\ live h b /\ exp_state_st_inv resLen aLen st h))
-    (ensures  (fun h0 _ h1 -> live h1 n /\ live h1 b /\ exp_state_st_inv resLen aLen st h1 /\
-                modifies_1 st h0 h1))
+    modBits:U32.t{U32.v modBits > 0} ->
+    aLen:U32.t{U32.v aLen > 0} -> 
+    bBits:U32.t{U32.v bBits > 0} -> 
+    resLen:U32.t{U32.v resLen > 0} ->
+    n:bignum{length n = U32.v (bits_to_bn modBits)} -> 
+    tmpV:bignum{length tmpV = U32.v aLen} -> 
+    b:bignum{length b = U32.v (bits_to_bn bBits)} ->
+    res:bignum{length res = U32.v resLen} ->
+    count:U32.t{U32.v count <= length b} -> Stack unit
+    (requires (fun h -> live h n /\ live h tmpV /\ live h b /\ live h res))
+    (ensures  (fun h0 _ h1 -> live h0 n /\ live h0 tmpV /\ live h0 b /\ live h0 res /\
+        live h1 n /\ live h1 tmpV /\ live h1 b /\ live h1 res /\ 
+        modifies_2 tmpV res h0 h1))
+let rec mod_exp_loop modBits aLen bBits resLen n tmpV b res count =
+    push_frame();
+    let tmpLen = U32.(2ul *^ aLen) in
+    let tmp = create 0uL tmpLen in
+    
+    let tmpLen2 = U32.(aLen +^ resLen) in
+    let tmp2 = create 0uL tmpLen2 in
+    let diffBits1 = U32.(64ul *^ 2ul *^ aLen -^ modBits) in
+    let diffBits2 = U32.(64ul *^ (aLen +^ resLen) -^ modBits) in
+    let modLen = bits_to_bn modBits in
 
-let rec mod_exp_loop modBits aLen bBits resLen n b count st =   
-    if U32.(count <^ bBits) then begin
-        let r_i = get_r_i st in
-        let tmp = get_tmp st in
-        let tmp2 = get_tmp2 st in
-        let r_itmp = get_r_itmp st in
-
-        let diffBits1 = U32.(64ul *^ 2ul *^ aLen -^ modBits) in
-        let diffBits2 = U32.(64ul *^ (aLen +^ resLen) -^ modBits) in
-        let modLen = bits_to_bn modBits in
-
-        (sqr aLen tmp tmp2;
-        Div.remainder U32.(2ul *^ aLen) modLen aLen diffBits1 tmp2 n tmp;
-        (if (bn_bit_is_set b count) then
-            (mult resLen aLen r_i tmp r_itmp;
-            Div.remainder U32.(aLen +^ resLen) modLen resLen diffBits2 r_itmp n r_i)));    
-        mod_exp_loop modBits aLen bBits resLen n b U32.(count +^ 1ul) st
-        end
-
+    (if U32.(count <^ bBits) then
+       (sqr aLen tmpV tmp;
+       remainder tmpLen modLen aLen diffBits1 tmp n tmpV;
+       (if (bn_bit_is_set b count) then
+           (mult resLen aLen res tmpV tmp2;
+            remainder tmpLen2 modLen resLen diffBits2 tmp2 n res));
+        let count = U32.(count +^ 1ul) in
+        mod_exp_loop modBits aLen bBits resLen n tmpV b res count));
+    pop_frame()
 
 (* res = a ^^ b mod n *)
 val mod_exp:
-    modBits:U32.t{U32.v modBits > 0} -> aLen:bnlen ->
-    bBits:U32.t{U32.v bBits > 0} -> resLen:bnlen ->
-    n:lbignum (bits_to_bn modBits) ->
-    a:lbignum aLen{disjoint a n} ->
-    b:lbignum (bits_to_bn bBits){disjoint b n /\ disjoint b a} ->
-    res:lbignum resLen{disjoint res n /\ disjoint res a /\ disjoint res b} -> Stack unit
+    modBits:U32.t{U32.v modBits > 0} ->
+    aLen:U32.t{U32.v aLen > 0} -> 
+    bBits:U32.t{U32.v bBits > 0} -> 
+    resLen:U32.t{U32.v resLen > 0} ->
+    n:bignum{length n = U32.v (bits_to_bn modBits)} ->
+    a:bignum{length a = U32.v aLen} ->
+    b:bignum{length b = U32.v (bits_to_bn bBits)} ->
+    res:bignum{length res = U32.v resLen} -> Stack unit
     (requires (fun h -> live h n /\ live h a /\ live h b /\ live h res))
     (ensures  (fun h0 _ h1 -> live h0 n /\ live h0 a /\ live h0 b /\ live h0 res /\
         live h1 n /\ live h1 a /\ live h1 b /\ live h1 res /\
         modifies_1 res h0 h1))
-
 let mod_exp modBits aLen bBits resLen n a b res =
     push_frame();
-    let st : exp_state resLen aLen = create 0uL U32.(resLen +^ aLen +^ (2ul *^ aLen) +^ (aLen +^ resLen)) in
-    let r_0 = get_r_i st in
-    let tmp = get_tmp st in
-    blit a 0ul tmp 0ul aLen;
+    let tmpV = create 0uL aLen in
+    blit a 0ul tmpV 0ul aLen;
 
-    (if (bn_bit_is_set b 0ul) then
-        blit a 0ul r_0 0ul aLen
-    else r_0.(0ul) <- 1uL);
+    if (bn_bit_is_set b 0ul) then
+        blit a 0ul res 0ul aLen
+    else res.(0ul) <- 1uL;
 
-    mod_exp_loop modBits aLen bBits resLen n b 1ul st;
-    blit r_0 0ul res 0ul resLen;
+    mod_exp_loop modBits aLen bBits resLen n b res tmpV 1ul;
     pop_frame()
